packages/mol-viewer/src/lib/modeling/relations/index.ts
@@ -1,0 +1,3 @@
+export * from './compiler'
+export * from './contracts'
+export * from './verifier'
